WIP: src/Slabs, try some admit fix

src/Slabs.fst
@@ -1229,6 +1229,20 @@ let allocate_slab_aux_3
   return r
 #pop-options
 
+let vp_aux
+  (slab_region: array U8.t{A.length slab_region = U32.v metadata_max * U32.v page_size})
+  (md_bm_region: array U64.t{A.length md_bm_region = U32.v metadata_max * 4})
+  (md_region: array SL.cell{A.length md_region = U32.v metadata_max})
+  (v: U32.t{U32.v v <= U32.v metadata_max == true})
+  : vprop
+  =
+  (A.varray (A.split_r slab_region (u32_to_sz (U32.mul v page_size)))
+    `vrefine` zf_u8) `star`
+  (A.varray (A.split_r md_bm_region (u32_to_sz (U32.mul v 4ul)))
+    `vrefine` zf_u64) `star`
+  A.varray (A.split_r md_region (u32_to_sz v))
+
+
 #push-options "--compat_pre_typed_indexed_effects --z3rlimit 100"
 let allocate_slab_check_md_count
   (slab_region: array U8.t{A.length slab_region = U32.v metadata_max * U32.v page_size})
@@ -1240,23 +1254,13 @@ let allocate_slab_check_md_count
     vrefinedep
       (vptr md_count)
       (fun x -> U32.v x <= U32.v metadata_max == true)
-      (fun v ->
-        (A.varray (A.split_r slab_region (u32_to_sz (U32.mul v page_size)))
-          `vrefine` zf_u8) `star`
-        (A.varray (A.split_r md_bm_region (u32_to_sz (U32.mul v 4ul)))
-          `vrefine` zf_u64) `star`
-        A.varray (A.split_r md_region (u32_to_sz v)))
+      (fun v -> vp_aux slab_region md_bm_region md_region v)
   )
   (fun _ ->
     vrefinedep
       (vptr md_count)
       (fun x -> U32.v x <= U32.v metadata_max == true)
-      (fun v ->
-        (A.varray (A.split_r slab_region (u32_to_sz (U32.mul v page_size)))
-          `vrefine` zf_u8) `star`
-        (A.varray (A.split_r md_bm_region (u32_to_sz (U32.mul v 4ul)))
-          `vrefine` zf_u64) `star`
-        A.varray (A.split_r md_region (u32_to_sz v)))
+      (fun v -> vp_aux slab_region md_bm_region md_region v)
   )
   (requires fun _ -> True)
   (ensures fun h0 r h1 ->
@@ -1264,22 +1268,14 @@ let allocate_slab_check_md_count
       = h0 (vrefinedep
       (vptr md_count)
       (fun x -> U32.v x <= U32.v metadata_max == true)
-      (fun v ->
-        (A.varray (A.split_r slab_region (u32_to_sz (U32.mul v page_size)))
-          `vrefine` zf_u8) `star`
-        (A.varray (A.split_r md_bm_region (u32_to_sz (U32.mul v 4ul)))
-          `vrefine` zf_u64) `star`
-        A.varray (A.split_r md_region (u32_to_sz v)))) in
+      (fun v -> vp_aux slab_region md_bm_region md_region v)
+    ) in
     let blob1
       = h1 (vrefinedep
       (vptr md_count)
       (fun x -> U32.v x <= U32.v metadata_max == true)
-      (fun v ->
-        (A.varray (A.split_r slab_region (u32_to_sz (U32.mul v page_size)))
-          `vrefine` zf_u8) `star`
-        (A.varray (A.split_r md_bm_region (u32_to_sz (U32.mul v 4ul)))
-          `vrefine` zf_u64) `star`
-        A.varray (A.split_r md_region (u32_to_sz v)))) in
+      (fun v -> vp_aux slab_region md_bm_region md_region v)
+    ) in
     blob0 == blob1 /\
     r == (U32.v (dfst blob0) < U32.v metadata_max)
   )
@@ -1287,48 +1283,25 @@ let allocate_slab_check_md_count
   let x0 = gget (vrefinedep
       (vptr md_count)
       (fun x -> U32.v x <= U32.v metadata_max == true)
-      (fun v ->
-        (A.varray (A.split_r slab_region (u32_to_sz (U32.mul v page_size)))
-          `vrefine` zf_u8) `star`
-        (A.varray (A.split_r md_bm_region (u32_to_sz (U32.mul v 4ul)))
-          `vrefine` zf_u64) `star`
-        A.varray (A.split_r md_region (u32_to_sz v)))) in
+      (fun v -> vp_aux slab_region md_bm_region md_region v)
+  ) in
   let x
     = elim_vrefinedep
     (vptr md_count)
     (fun x -> U32.v x <= U32.v metadata_max == true)
-    (fun v ->
-      (A.varray (A.split_r slab_region (u32_to_sz (U32.mul v page_size)))
-        `vrefine` zf_u8) `star`
-      (A.varray (A.split_r md_bm_region (u32_to_sz (U32.mul v 4ul)))
-        `vrefine` zf_u64) `star`
-      A.varray (A.split_r md_region (u32_to_sz v)))
+    (fun v -> vp_aux slab_region md_bm_region md_region v)
   in
   let r = read md_count in
-  admit ();
   intro_vrefinedep
     (vptr md_count)
     (fun x -> U32.v x <= U32.v metadata_max == true)
-    (fun v ->
-      (A.varray (A.split_r slab_region (u32_to_sz (U32.mul v page_size)))
-        `vrefine` zf_u8) `star`
-      (A.varray (A.split_r md_bm_region (u32_to_sz (U32.mul v 4ul)))
-        `vrefine` zf_u64) `star`
-      A.varray (A.split_r md_region (u32_to_sz v)))
-    ((A.varray (A.split_r slab_region (u32_to_sz (U32.mul (G.reveal x) page_size)))
-      `vrefine` zf_u8) `star`
-    (A.varray (A.split_r md_bm_region (u32_to_sz (U32.mul (G.reveal x) 4ul)))
-      `vrefine` zf_u64) `star`
-    A.varray (A.split_r md_region (u32_to_sz (G.reveal x))));
+    (fun v -> vp_aux slab_region md_bm_region md_region v)
+    (vp_aux slab_region md_bm_region md_region (G.reveal x));
   let x1 = gget (vrefinedep
       (vptr md_count)
       (fun x -> U32.v x <= U32.v metadata_max == true)
-      (fun v ->
-        (A.varray (A.split_r slab_region (u32_to_sz (U32.mul v page_size)))
-          `vrefine` zf_u8) `star`
-        (A.varray (A.split_r md_bm_region (u32_to_sz (U32.mul v 4ul)))
-          `vrefine` zf_u64) `star`
-        A.varray (A.split_r md_region (u32_to_sz v)))) in
+      (fun v -> vp_aux slab_region md_bm_region md_region v)
+  ) in
   assert (dfst x0 == dfst x1);
   assert (dsnd x0 == dsnd x1);
   return (U32.lt r metadata_max)
